add --input_stream option (buffer|extern)

src/3d/ocaml/Batch.ml
@@ -10,8 +10,8 @@ let lowparse_home = filename_concat (filename_concat qd_home "src") "lowparse"
 let ddd_home = filename_concat (filename_concat qd_home "src") "3d"
 let ddd_prelude_home = filename_concat (filename_concat (filename_concat qd_home "src") "3d") "prelude"
 
-let ddd_actions_home () =
-  filename_concat ddd_prelude_home "buffer"
+let ddd_actions_home input_stream_binding =
+  filename_concat ddd_prelude_home (string_of_input_stream_binding input_stream_binding)
 
 (* fstar.exe executable *)
 let fstar_exe = (filename_concat (filename_concat fstar_home "bin") "fstar.exe")
@@ -67,45 +67,50 @@ let list_snoc q a =
   q @ [a]
 
 let fstar_args
+  input_stream_binding
   out_dir
 =
     "--odir" :: out_dir ::
       "--cache_dir" :: out_dir ::
-        "--include" :: ddd_actions_home () ::
+        "--include" :: ddd_actions_home input_stream_binding ::
         "--include" :: out_dir ::
           "--load_cmxs" :: "WeakenTac" ::
             fstar_args0
 
 let verify_fst_file
+  input_stream_binding
   out_dir
   file
 =
-  let fstar_args = list_snoc (fstar_args out_dir) file in
+  let fstar_args = list_snoc (fstar_args input_stream_binding out_dir) file in
   run_cmd fstar_exe ("--cache_checked_modules" :: fstar_args)
 
 let fstar_modul_of_filename fst =
   let basename = remove_extension (basename fst) in
   String.concat "." (List.map String.capitalize_ascii (String.split_on_char '.' basename))
 
-let fstar_extract_args out_dir fst =
+let fstar_extract_args input_stream_binding out_dir fst =
   "--extract_module" :: fstar_modul_of_filename fst ::
     "--codegen" :: "Kremlin" ::
-      (list_snoc (fstar_args out_dir) fst)
+      (list_snoc (fstar_args input_stream_binding out_dir) fst)
 
 let extract_fst_file
+  input_stream_binding
   out_dir
   file
 =
-  run_cmd fstar_exe (fstar_extract_args out_dir file)
+  run_cmd fstar_exe (fstar_extract_args input_stream_binding out_dir file)
 
 let pretty_print_source_file
+  input_stream_binding
   out_dir
   file
 =
-  let fstar_args = list_snoc (fstar_args out_dir) file in
+  let fstar_args = list_snoc (fstar_args input_stream_binding out_dir) file in
   run_cmd fstar_exe ("--print_in_place" :: fstar_args)
 
 let pretty_print_source_module
+      input_stream_binding
       out_dir
       (file, modul)
     : unit
@@ -113,19 +118,21 @@ let pretty_print_source_module
   let fst_file = filename_concat out_dir (Printf.sprintf "%s.fst" modul) in
   let types_fst_file = filename_concat out_dir (Printf.sprintf "%s.Types.fst" modul) in
   let fsti_file = Printf.sprintf "%si" fst_file in
-  List.iter (pretty_print_source_file out_dir) [
+  List.iter (pretty_print_source_file input_stream_binding out_dir) [
       types_fst_file;
       fsti_file;
       fst_file;
   ]
 
 let pretty_print_source_modules
+      input_stream_binding
       (out_dir: string)
       (files_and_modules: (string * string) list)
 =
-  List.iter (pretty_print_source_module out_dir) files_and_modules
+  List.iter (pretty_print_source_module input_stream_binding out_dir) files_and_modules
 
 let verify_and_extract_module
+      input_stream_binding
       out_dir
       (file, modul)
     : unit
@@ -133,12 +140,12 @@ let verify_and_extract_module
   let fst_file = filename_concat out_dir (Printf.sprintf "%s.fst" modul) in
   let types_fst_file = filename_concat out_dir (Printf.sprintf "%s.Types.fst" modul) in
   let fsti_file = Printf.sprintf "%si" fst_file in
-  List.iter (verify_fst_file out_dir) [
+  List.iter (verify_fst_file input_stream_binding out_dir) [
       types_fst_file;
       fsti_file;
       fst_file;
   ];
-  List.iter (extract_fst_file out_dir) [
+  List.iter (extract_fst_file input_stream_binding out_dir) [
       types_fst_file;
       fst_file;
   ]
@@ -167,9 +174,9 @@ let all_krmls_in_dir
     Unix.closedir h;
     res
 
-let all_everparse_krmls () =
+let all_everparse_krmls input_stream_binding =
   let prelude = all_krmls_in_dir ddd_prelude_home in
-  let actions = all_krmls_in_dir (ddd_actions_home ()) in
+  let actions = all_krmls_in_dir (ddd_actions_home input_stream_binding) in
   let actions_base = List.map basename actions in
   let prelude' = List.filter (fun f -> not (List.mem (basename f) actions_base)) prelude in
   prelude' @ actions
@@ -194,7 +201,7 @@ let everparse_only_bundle = "Prims,LowParse.\\*,EverParse3d.\\*,ResultOps,Prelud
 
 let fstar_kremlib_bundle = "FStar.\\*,LowStar.\\*,C.\\*"
 
-let krml_args skip_c_makefiles out_dir files_and_modules =
+let krml_args input_stream_binding skip_c_makefiles out_dir files_and_modules =
   let krml_files = List.fold_left
                      (fun accu (_, modul) ->
                        let l =
@@ -215,7 +222,7 @@ let krml_args skip_c_makefiles out_dir files_and_modules =
                          else l in
 		       l
                      )
-                     (all_everparse_krmls ())
+                     (all_everparse_krmls input_stream_binding)
                      files_and_modules
   in
   let krml_files = List.rev krml_files in
@@ -274,13 +281,14 @@ let call_krml files_and_modules_cleanup out_dir krml_args =
   end
 
 let produce_c_files
+      input_stream_binding
       (skip_c_makefiles: bool)
       (cleanup: bool)
       (out_dir: string)
       (files_and_modules: (string * string) list)
     : unit
   =
-  let krml_args = krml_args skip_c_makefiles out_dir files_and_modules in
+  let krml_args = krml_args input_stream_binding skip_c_makefiles out_dir files_and_modules in
   (* bundle M.Types.krml and EverParse into M *)
   let krml_args =
     let bundle_types = List.fold_left (fun acc (_, modul) ->
@@ -292,13 +300,14 @@ let produce_c_files
   call_krml (if cleanup then Some files_and_modules else None) out_dir krml_args
 
 let produce_one_c_file
+      input_stream_binding
       (out_dir: string)
       (file: string)
       (modul: string)
       (dep_files_and_modules: (string * string) list)
     : unit
   =
-  let krml_args = krml_args true out_dir ((file, modul) :: dep_files_and_modules) in
+  let krml_args = krml_args input_stream_binding true out_dir ((file, modul) :: dep_files_and_modules) in
   let krml_args =
     krml_args@
       List.concat (List.map (fun (_, m) -> ["-library"; Printf.sprintf "%s,%s.Types" m m]) dep_files_and_modules) @ [
@@ -544,6 +553,7 @@ let copy_clang_format out_dir =
 (* Postprocess C files, assuming that they have already been processed *)
 
 let postprocess_c
+      input_stream_binding
       (produced_files: bool)
       (wrappers: bool)
       (clang_format: bool)
@@ -561,7 +571,7 @@ let postprocess_c
   if not no_everparse_h
   then begin
       let dest_everparse_h = filename_concat out_dir "EverParse.h" in
-      copy (filename_concat (ddd_actions_home ()) "EverParse.h") dest_everparse_h;
+      copy (filename_concat (ddd_actions_home input_stream_binding) "EverParse.h") dest_everparse_h;
       copy (filename_concat ddd_home (Printf.sprintf "EverParseEndianness%s.h" (if Sys.win32 then "_Windows_NT" else ""))) (filename_concat out_dir "EverParseEndianness.h")
     end;
   (* clang-format the files if asked for *)
@@ -583,6 +593,7 @@ let postprocess_c
   ()
 
 let produce_and_postprocess_c
+      input_stream_binding
       (clang_format: bool)
       (clang_format_executable: string)
       (skip_c_makefiles: bool)
@@ -595,13 +606,14 @@ let produce_and_postprocess_c
   =
   let everparse_h_existed_before = Sys.file_exists (filename_concat out_dir "EverParse.h") in
   (* produce the C files *)
-  produce_c_files skip_c_makefiles cleanup out_dir files_and_modules;
+  produce_c_files input_stream_binding skip_c_makefiles cleanup out_dir files_and_modules;
   if Sys.file_exists (filename_concat out_dir "EverParse.h") && not everparse_h_existed_before
   then failwith "krml produced some EverParse.h, should not have happened";
   (* postprocess the produced C files *)
-  postprocess_c true true clang_format clang_format_executable true skip_c_makefiles cleanup no_everparse_h save_hashes_opt out_dir files_and_modules
+  postprocess_c input_stream_binding true true clang_format clang_format_executable true skip_c_makefiles cleanup no_everparse_h save_hashes_opt out_dir files_and_modules
 
 let produce_and_postprocess_one_c
+      input_stream_binding
       (clang_format: bool)
       (clang_format_executable: string)
       (out_dir: string)
@@ -612,22 +624,24 @@ let produce_and_postprocess_one_c
   =
   let everparse_h_existed_before = Sys.file_exists (filename_concat out_dir "EverParse.h") in
   (* produce the .c and .h file *)
-  produce_one_c_file out_dir file modul dep_files_and_modules;
+  produce_one_c_file input_stream_binding out_dir file modul dep_files_and_modules;
   if Sys.file_exists (filename_concat out_dir "EverParse.h") && not everparse_h_existed_before
   then failwith "krml produced some EverParse.h, should not have happened";
   (* postprocess the produced .c and .h files for this module *)
-  postprocess_c true false clang_format clang_format_executable false true false true false out_dir [file, modul]
+  postprocess_c input_stream_binding true false clang_format clang_format_executable false true false true false out_dir [file, modul]
 
 let postprocess_wrappers
+      input_stream_binding
       (clang_format: bool)
       (clang_format_executable: string)
       (out_dir: string)
       (files_and_modules: (string * string) list)
     : unit
   =
-  postprocess_c false true clang_format clang_format_executable false true false true false out_dir files_and_modules
+  postprocess_c input_stream_binding false true clang_format clang_format_executable false true false true false out_dir files_and_modules
 
 let postprocess_fst
+      input_stream_binding
       (clang_format: bool)
       (clang_format_executable: string)
       (skip_c_makefiles: bool)
@@ -640,9 +654,9 @@ let postprocess_fst
   =
   (* produce the .checked and .krml files.
      FIXME: modules can be processed in parallel *)
-  List.iter (verify_and_extract_module out_dir) files_and_modules;
+  List.iter (verify_and_extract_module input_stream_binding out_dir) files_and_modules;
   (* produce the .c and .h files and format them *)
-  produce_and_postprocess_c clang_format clang_format_executable skip_c_makefiles cleanup no_everparse_h save_hashes_opt out_dir files_and_modules
+  produce_and_postprocess_c input_stream_binding clang_format clang_format_executable skip_c_makefiles cleanup no_everparse_h save_hashes_opt out_dir files_and_modules
 
 let check_all_hashes
       (ch: check_hashes_t)
